Paxos/ExtraLemma.lean
@@ -11,34 +11,32 @@ namespace Paxos.ExtraLemma
 open Paxos.Spec Paxos.Prop
 open Set Classical
 
-variable (Quorums: Set (Set Acceptor))
-variable (sent sent': Set Message)
+variable (Quorums : Set (Set Acceptor))
+variable (sent sent' : Set Message)
 
--- The following four are helper definitions for checking message types.
-
+-- Helper definitions for checking message types.
 @[simp] def is1a : Message → Prop | Message.onea _ => True | _ => False
 @[simp] def is1b : Message → Prop | Message.oneb _ _ _ _ => True | _ => False
 @[simp] def is2a : Message → Prop | Message.twoa _ _ => True | _ => False
 @[simp] def is2b : Message → Prop | Message.twob _ _ _ => True | _ => False
 
-/-- Used in proving that Phase2a is inductive. -/
+/-- `none + 1 ≤ some b` for any ballot `b`. Used in showing inductiveness for `Phase2a`. -/
 @[simp]
-lemma ballot_none_plus_one_leq_ballot
-    {b : Ballot} : (none : Option Ballot) + (1 : Nat) ≤ some b := by
+lemma ballot_none_plus_one_leq_ballot {b : Ballot} :
+    (none : Option Ballot) + (1 : Nat) ≤ some b := by
   dsimp [HAdd.hAdd]
   exact Nat.zero_le b
 
 /-- The immediate consequence of `QuorumAssumption`. Used to pick an witness from the
 intersection of two quorums. -/
-@[simp]
 lemma pick_from_quorum_int {Q₁ Q₂ : Set Acceptor}
-    (h1: Q₁ ∈ Quorums)
-    (h2: Q₂ ∈ Quorums) : ∃ a: Acceptor, a ∈ Q₁ ∩ Q₂ := by
+    (h1 : Q₁ ∈ Quorums)
+    (h2 : Q₂ ∈ Quorums) : ∃ a : Acceptor, a ∈ Q₁ ∩ Q₂ := by
   have hne := QuorumAssumption Quorums h1 h2
   rcases ((Iff.mpr nonempty_iff_ne_empty) hne) with ⟨aa, haa⟩
   exact Exists.intro aa haa
 
-/-- Transitive property of `Option Ballot`. Used in `ind_phase2a`. -/
+/-- Transitive property of `Option Ballot`. Used in showing inductiveness for `Phase2a`. -/
 @[simp]
 lemma option.some_succ_le_some_of_some_le_and_lt {n m k : Ballot}
     (h₁ : some n ≤ some m)
@@ -93,9 +91,9 @@ lemma max_prop_empty_ballot_iff_empty_value {a : Acceptor} {m : Message}
 /-- The acceptor could not have voted for a ballot greater than the one in `max_prop` -/
 @[simp]
 lemma max_prop_implies_not_voted_for_greater_ballots
-    {a : Acceptor} {b : Ballot} {v: Value} :
+    {a : Acceptor} {b : Ballot} {v : Value} :
     Message.twob b (some v) a ∈ max_prop sent a →
-      ∀ b', b' ≥ b+1 → ¬∃ v, VotedForIn sent a v b' := by
+      ∀ b', b' ≥ b + 1 → ¬∃ v, VotedForIn sent a v b' := by
   intro h_mem
   unfold max_prop at h_mem
   simp at h_mem
@@ -117,9 +115,9 @@ lemma max_prop_implies_not_voted_for_greater_ballots
 voted in any previous ballots. Used in proving the case when both `rbal` and `rval` are
 empty in the proof of `Phase1b`. -/
 @[simp]
-lemma max_prop_empty_implies_not_voted_in_prev_ballots {a: Acceptor}
-    (hm: Message.twob none none a ∈ max_prop sent a) :
-    ∀ b, ∀ (v: Value), ¬ VotedForIn sent a v b := by
+lemma max_prop_empty_implies_not_voted_in_prev_ballots {a : Acceptor}
+    (hm : Message.twob none none a ∈ max_prop sent a) :
+    ∀ b, ∀ (v : Value), ¬ VotedForIn sent a v b := by
   intro b' hb'_le h_voted
   unfold max_prop at hm
   simp [*] at *
@@ -140,46 +138,39 @@ lemma max_prop_empty_implies_not_voted_in_prev_ballots {a: Acceptor}
 /--The immediate consequence of the definition of `Send`. We use this lemma to show that
 `Next` grows the history variable `sent` monotonically. -/
 @[simp]
-lemma send_monotonic {sent sent': Set Message} {x: Message}
-    (h: sent' = Send x sent) : sent ⊆ sent' := by
+lemma send_monotonic {sent sent' : Set Message} {x : Message}
+    (h : sent' = Send x sent) : sent ⊆ sent' := by
   simp [Send, h]
 
 /-- `Phase1a` grows `sent` monotonically. -/
 @[simp]
-lemma phase1a_imp_mono_sent {b: Ballot}
-    (hPhase1a: Phase1a sent sent' b) : sent ⊆ sent' := by
+lemma phase1a_imp_mono_sent {b : Ballot} {sent sent' : Set Message}
+    (hPhase1a : Phase1a sent sent' b) : sent ⊆ sent' := by
   exact send_monotonic hPhase1a
 
 /-- `Phase1b` grows `sent` monotonically. -/
 @[simp]
-lemma phase1b_imp_mono_sent {a: Acceptor}
-    (hPhase1b: Phase1b sent sent' a) : sent ⊆ sent' := by
+lemma phase1b_imp_mono_sent {a : Acceptor} {sent sent' : Set Message}
+    (hPhase1b : Phase1b sent sent' a) : sent ⊆ sent' := by
   rcases hPhase1b with ⟨m, hm, r, hr, hmatch⟩
   cases m <;> cases r <;> simp at hmatch; simp [hmatch]
 
 /-- `Phase2a` grows `sent` monotonically. -/
 @[simp]
-lemma phase2a_imp_mono_sent {b: Ballot}
-    (hPhase2a: Phase2a Quorums sent sent' b) : sent ⊆ sent' := by
+lemma phase2a_imp_mono_sent {b : Ballot} {sent sent' : Set Message} {Quorums : Set (Set Acceptor)}
+    (hPhase2a : Phase2a Quorums sent sent' b) : sent ⊆ sent' := by
   rcases hPhase2a with ⟨h_no_2a, ⟨_, _, _, h_rest⟩⟩
   simp [h_rest]
 
 /-- `Phase2b` grows `sent` monotonically. -/
 @[simp]
-lemma phase2b_imp_mono_sent {a: Acceptor}
-    (hPhase2b: Phase2b sent sent' a) : sent ⊆ sent' := by
+lemma phase2b_imp_mono_sent {a : Acceptor} {sent sent' : Set Message}
+    (hPhase2b : Phase2b sent sent' a) : sent ⊆ sent' := by
   rcases hPhase2b with ⟨m2b, hm2b, hmatch⟩
   cases m2b <;> simp at hmatch; simp [hmatch]
 
-/-- `sent` grows monotonically with `Next`. Used in the proof of `SafeAtStable`. -/
-@[simp]
-lemma next_imp_mono_sent
-    (hNext: Next Quorums sent sent') : sent ⊆ sent' := by
-  rcases hNext with ⟨b, hPhase1a | hPhase2a⟩ | ⟨a, hPhase1b | hPhase2b⟩
-  · exact phase1a_imp_mono_sent sent sent' hPhase1a
-  · exact phase2a_imp_mono_sent Quorums sent sent' hPhase2a
-  · exact phase1b_imp_mono_sent sent sent' hPhase1b
-  · exact phase2b_imp_mono_sent sent sent' hPhase2b
+-- Lemmas about monotonicity of `VotedForIn` and `WontVoteIn`. We use word "stable" to mean
+-- implication, and "same" to mean if and only if.
 
 /-- The monotonicity of existantial quantifier describe in the TLAPS proof. -/
 lemma exists_mem_of_subset {s t : Set Message} {P : Message → Prop}
@@ -189,14 +180,14 @@ lemma exists_mem_of_subset {s t : Set Message} {P : Message → Prop}
 
 /-- If `sent` is a subset of `sent'`, then voted in the former implies voted in the latter.
 Used in the proof of `SafeAtStable`.-/
-lemma votedForIn_monotonic
-    (h1: sent ⊆ sent') : VotedForIn sent a v b → VotedForIn sent' a v b := by
+lemma votedForIn_stable
+    (h1 : sent ⊆ sent') : VotedForIn sent a v b → VotedForIn sent' a v b := by
   exact exists_mem_of_subset h1
 
 /-- If no 2b message is added, then the value of `VotedForIn` stays the same. -/
 lemma votedForIn_same_if_no_2b_added
-    (h_mono: sent ⊆ sent')
-    (hm: ∀ m ∈ sent' \ sent, ¬ is2b m) :
+    (h_mono : sent ⊆ sent')
+    (hm : ∀ m ∈ sent' \ sent, ¬ is2b m) :
     VotedForIn sent a v b ↔ VotedForIn sent' a v b := by
   unfold VotedForIn at *
   constructor
@@ -218,26 +209,25 @@ lemma votedForIn_same_if_no_2b_send
   exact votedForIn_same_if_no_2b_added sent sent' h_mono h_no_2b_added
 
 /-- If no 1b or 2b message is added, then the second invariant for 2b is stable. -/
-lemma oneb_inv_2_stable_if_no_twob_added {maxVBal: Option Ballot} {b: Ballot} {a: Acceptor}
+lemma oneb_inv_2_stable_if_no_twob_added {maxVBal : Option Ballot} {b : Ballot} {a : Acceptor}
     (sent sent': Set Message)
-    (h_mono: sent ⊆ sent')
-    (h_no_2b_added: ∀ m ∈ sent' \ sent, ¬ is2b m) :
-    (∀ (b' : Ballot), (b' ≥ (maxVBal + (1: Nat)) ∧ (b' < b))
-          → ¬(∃ v : Value, VotedForIn sent a v b')) →
-    (∀ (b' : Ballot), (b' ≥ (maxVBal + (1: Nat)) ∧ (b' < b))
-          → ¬(∃ v : Value, VotedForIn sent' a v b')) := by
+    (h_mono : sent ⊆ sent')
+    (h_no_2b_added : ∀ m ∈ sent' \ sent, ¬ is2b m) :
+    (∀ (b' : Ballot), (b' ≥ (maxVBal + (1 : Nat)) ∧ (b' < b))
+      → ¬(∃ v : Value, VotedForIn sent a v b')) →
+    (∀ (b' : Ballot), (b' ≥ (maxVBal + (1 : Nat)) ∧ (b' < b))
+      → ¬(∃ v : Value, VotedForIn sent' a v b')) := by
   intro h_not_voted_in_sent b' hle ⟨v, h_voted_in_sent'⟩
   have h_no_vote_in_sent_b' := h_not_voted_in_sent b' hle
   simp at h_no_vote_in_sent_b'
   exact h_no_vote_in_sent_b' v
-          ((votedForIn_same_if_no_2b_added sent sent' h_mono h_no_2b_added).mpr
-          h_voted_in_sent')
+    ((votedForIn_same_if_no_2b_added sent sent' h_mono h_no_2b_added).mpr h_voted_in_sent')
 
 /-- If no 1b or 2b message is added, then `WontVoteIn` is stable. -/
 lemma wontVoteIn_stable_if_no_1b2b_added
-    (h_mono: sent ⊆ sent')
-    (hm: ∀ m ∈ sent' \ sent, ¬ (is1b m ∨ is2b m)) :
-    WontVoteIn sent a b → WontVoteIn sent' a b := by
+    (h_mono : sent ⊆ sent')
+    (hm : ∀ m ∈ sent' \ sent, ¬ (is1b m ∨ is2b m)) :
+  WontVoteIn sent a b → WontVoteIn sent' a b := by
   unfold WontVoteIn
   intro h_wontVoteIn_sent
   rcases h_wontVoteIn_sent with ⟨h_no_vote, h_exists_greater_ballot⟩
@@ -245,7 +235,7 @@ lemma wontVoteIn_stable_if_no_1b2b_added
   · intro v h_voted_in_sent'; specialize h_no_vote v
     have h_no_2b_added : ∀ m' ∈ sent' \ sent, ¬ is2b m' := by simp_all
     simp [@votedForIn_same_if_no_2b_added sent sent' a v b h_mono h_no_2b_added,
-          h_voted_in_sent'] at h_no_vote
+      h_voted_in_sent'] at h_no_vote
   · exact exists_mem_of_subset h_mono h_exists_greater_ballot
 
 end Paxos.ExtraLemma
